NT --> Nt

GNF.thy
@@ -11,12 +11,12 @@ definition rtps :: "('n,'t)prodS \<Rightarrow> bool" where
 "rtps ps = (\<forall>p \<in> ps. rt(snd p))"
 
 definition Lnt :: "('n, 't) prodS \<Rightarrow> ('n * 'n * ('n,'t)syms)set" where
-"Lnt P = {(A,B,w). (A, NT B # w) \<in> P}"
+"Lnt P = {(A,B,w). (A, Nt B # w) \<in> P}"
 
-lemma [code]: "Lnt P = \<Union> ((\<lambda>(A,w). case w of NT B#v \<Rightarrow> {(A,B,v)} | _ \<Rightarrow> {}) ` P)"
+lemma [code]: "Lnt P = \<Union> ((\<lambda>(A,w). case w of Nt B#v \<Rightarrow> {(A,B,v)} | _ \<Rightarrow> {}) ` P)"
   by (auto simp: Lnt_def split: list.splits sym.splits)
 
-definition rule where "rule = (\<lambda>(A, B, w). (A, NT B # w))"
+definition rule where "rule = (\<lambda>(A, B, w). (A, Nt B # w))"
 
 lemma Lnt_Un: "Lnt (A \<union> B) = Lnt A \<union> Lnt B"
 by(auto simp: Lnt_def)
@@ -29,10 +29,10 @@ by(auto simp: Lnt_def rule_def image_def split:prod.splits)
 
 (*
 fun lnt :: "('n,'t)prod \<Rightarrow> 'n option" where
-"lnt(_,NT A # _) = Some A" |
+"lnt(_,Nt A # _) = Some A" |
 "lnt _ = None"
 
-definition "has_lnt p = (\<exists>A u. snd p = NT A # u)"
+definition "has_lnt p = (\<exists>A u. snd p = Nt A # u)"
 
 lemma has_lnt_iff_lnt_split_Some: "has_lnt p = (\<exists>A. lnt_split p = Some A)"
 by(cases p rule: lnt_split.cases) (auto simp: has_lnt_def)
@@ -70,7 +70,7 @@ definition "Rhs1 R = rhs1 ` Lnt R"
 lemma lem: "A - {x. P x} = {x\<in>A. \<not>P x}"
 by auto
 
-lemma Rhs1_subsetD: "Rhs1 R \<subseteq> M \<Longrightarrow> (A, NT B # w) \<in> R \<Longrightarrow> B \<in> M"
+lemma Rhs1_subsetD: "Rhs1 R \<subseteq> M \<Longrightarrow> (A, Nt B # w) \<in> R \<Longrightarrow> B \<in> M"
 sorry
 
 lemma Lnt_subset: "R \<subseteq> S \<Longrightarrow> Lnt R \<subseteq> Lnt S"
@@ -84,20 +84,20 @@ lemma Rhs1_Un: "Rhs1 (R \<union> S) = Rhs1 R \<union> Rhs1 S"
 
 fun starts_with where
   "starts_with _ [] = False" |
-  "starts_with A (a # w) \<longleftrightarrow> a = NT A"
+  "starts_with A (a # w) \<longleftrightarrow> a = Nt A"
 
-lemma starts_with_iff: "starts_with A w \<longleftrightarrow> (\<exists>v. w = NT A # v)"
+lemma starts_with_iff: "starts_with A w \<longleftrightarrow> (\<exists>v. w = Nt A # v)"
   apply (cases "(A,w)" rule: starts_with.cases) by auto
 
-definition "ends_with A w = (\<exists>v. w = v @ [NT A])"
+definition "ends_with A w = (\<exists>v. w = v @ [Nt A])"
 
 lemma ends_with_iff_starts_with_rev: "ends_with A w \<longleftrightarrow> starts_with A (rev w)"
   apply (auto simp: starts_with_iff ends_with_def)
   by (metis rev_rev_ident)
 
-definition "loop R A = {(A,NT A # w) | w. (A, NT A # w) \<in> R \<and> w \<noteq> []}"
+definition "loop R A = {(A,Nt A # w) | w. (A, Nt A # w) \<in> R \<and> w \<noteq> []}"
 
-definition "right_loop R A = {(A,w@[NT A]) | w. (A, w@[NT A]) \<in> R \<and> w \<noteq> []}"
+definition "right_loop R A = {(A,w@[Nt A]) | w. (A, w@[Nt A]) \<in> R \<and> w \<noteq> []}"
 
 lemma right_loop_eq_loop:
   "right_loop R A = map_prod id rev ` loop (map_prod id rev ` R) A"
@@ -109,7 +109,7 @@ lemma loop_freeI:
   assumes "\<And>w. (A,w) \<in> R \<Longrightarrow> \<not>starts_with A w" shows "loop_free R A"
   using assms by (auto simp: loop_free_def)
 
-lemma loop_freeD: "loop_free R A \<Longrightarrow> (A, NT A # w) \<notin> R"
+lemma loop_freeD: "loop_free R A \<Longrightarrow> (A, Nt A # w) \<notin> R"
   by (auto simp: loop_free_def)
 
 definition "loop_free_list R A = (\<forall>(B,w) \<in> set R. B = A \<longrightarrow> \<not> starts_with A w)"
@@ -132,19 +132,19 @@ lemma solved: "solved (set R) (set As) = solved_list R As"
   by (auto simp: solved_def solved_list_def)
 
 lemma solved_not:
-  "solved R As \<Longrightarrow> A \<in> As \<Longrightarrow> (B,NT A#w) \<notin> R"
+  "solved R As \<Longrightarrow> A \<in> As \<Longrightarrow> (B,Nt A#w) \<notin> R"
   by (fastforce simp: solved_def starts_with_iff split: prod.splits)
 
-definition Nts where "Nts R = concat [A#[B. NT B \<leftarrow> w]. (A,w) \<leftarrow> R]"
+definition nonterminals where "nonterminals R = concat [A#[B. Nt B \<leftarrow> w]. (A,w) \<leftarrow> R]"
 
-definition Nt where "Nt R = (\<Union>(A,w)\<in>R. {A}\<union>{B. NT B \<in> set w})"
+definition Nonterminal where "Nonterminal R = (\<Union>(A,w)\<in>R. {A}\<union>{B. Nt B \<in> set w})"
 
 fun hdnt where
-    "hdnt (NT A#w) = Some A"
+    "hdnt (Nt A#w) = Some A"
   | "hdnt _ = None"
 
-lemma set_Nts_def: "set (Nts R) = Nt (set R)"
-  by (auto simp: Nts_def Nt_def)
+lemma set_nonterminals_def: "set (nonterminals R) = Nonterminal (set R)"
+  by (auto simp: nonterminals_def Nonterminal_def)
 
 definition "diff_list = fold removeAll"
 
@@ -153,11 +153,11 @@ lemma set_diff_list[simp]: "set(diff_list xs ys) = set ys - set xs"
 
 definition unwind_new where
   "unwind_new R A A' = (
-  \<Union>{{(A',w), (A',w@[NT A'])} | w. (A,NT A # w) \<in> R \<and> w \<noteq> []})"
+  \<Union>{{(A',w), (A',w@[Nt A'])} | w. (A,Nt A # w) \<in> R \<and> w \<noteq> []})"
 
 definition unwind_new_list where
   "unwind_new_list R A A' =
-  concat [[(A',w), (A',w@[NT A'])]. (B,NT C # w) \<leftarrow> R, B = A \<and> C = A \<and> w \<noteq> []]"
+  concat [[(A',w), (A',w@[Nt A'])]. (B,Nt C # w) \<leftarrow> R, B = A \<and> C = A \<and> w \<noteq> []]"
 
 lemma set_unwind_new_list: "set (unwind_new_list R A A') = unwind_new (set R) A A'"
   apply (auto simp: unwind_new_list_def unwind_new_def starts_with_iff)
@@ -166,14 +166,14 @@ lemma set_unwind_new_list: "set (unwind_new_list R A A') = unwind_new (set R) A 
 
 definition unwind_old where
   "unwind_old R A A' = (
-  let X = {(A, NT A # w) | w. (A, NT A # w) \<in> R} in
-  R - X \<union> {(A, w@[NT A']) |w. (A,w) \<in> R - X})"
+  let X = {(A, Nt A # w) | w. (A, Nt A # w) \<in> R} in
+  R - X \<union> {(A, w@[Nt A']) |w. (A,w) \<in> R - X})"
 
 definition unwind_old_list where
   "unwind_old_list R A A' = (
   let X = [(B,w) \<leftarrow> R. B = A \<and> starts_with A w] in
   diff_list X R @
-  [(A, w@[NT A']). (B,w) \<leftarrow> R, B = A \<and> \<not> starts_with A w])"
+  [(A, w@[Nt A']). (B,w) \<leftarrow> R, B = A \<and> \<not> starts_with A w])"
 
 lemma set_unwind_old_list: "set (unwind_old_list R A A') = unwind_old (set R) A A'"
   by (auto simp: unwind_old_def unwind_old_list_def starts_with_iff)
@@ -194,34 +194,34 @@ definition unwind_old_expand_list where
   "unwind_old_expand_list R A A' = (
   let X = [(B,w) \<leftarrow> R. starts_with A w] in
   diff_list X R @
-  [(A, w@[NT A']). (B,w) \<leftarrow> R, B = A \<and> \<not> starts_with A w] @
-  concat [[(B,w@tl v),(B,w@NT A'#tl v)]. (B,v) \<leftarrow> R, (C,w) \<leftarrow> diff_list X R, starts_with A v \<and> A \<noteq> B \<and> C = A ])"
+  [(A, w@[Nt A']). (B,w) \<leftarrow> R, B = A \<and> \<not> starts_with A w] @
+  concat [[(B,w@tl v),(B,w@Nt A'#tl v)]. (B,v) \<leftarrow> R, (C,w) \<leftarrow> diff_list X R, starts_with A v \<and> A \<noteq> B \<and> C = A ])"
 
 definition unwind_old_expand where
   "unwind_old_expand R A A' = (
-  let X = {(B, NT A # w) | B w. (B, NT A # w) \<in> R} in
-  R - X \<union> {(A, w @ [NT A']) |w. (A,w) \<in> R - X} \<union>
-  \<Union>{{(B, w@v), (B, w @ NT A' # v)} |B v w.
- (B, NT A # v) \<in> R \<and> A \<noteq> B \<and> (A,w) \<in> R - X })"
+  let X = {(B, Nt A # w) | B w. (B, Nt A # w) \<in> R} in
+  R - X \<union> {(A, w @ [Nt A']) |w. (A,w) \<in> R - X} \<union>
+  \<Union>{{(B, w@v), (B, w @ Nt A' # v)} |B v w.
+ (B, Nt A # v) \<in> R \<and> A \<noteq> B \<and> (A,w) \<in> R - X })"
 
 lemma set_unwind_old_expand_list: "set (unwind_old_expand_list R A A') = unwind_old_expand (set R) A A'"
   apply (auto simp: unwind_old_expand_def unwind_old_expand_list_def starts_with_iff)
   sorry
 
 definition "expand R S As =
-  {(A, b # w) |A b w. (A, b # w) \<in> R \<and> b \<notin> NT ` As} \<union>
-  {(A,v@w) |A v w. \<exists>B \<in> As. (A,NT B # w) \<in> R \<and> (B,v) \<in> S}"
+  {(A, b # w) |A b w. (A, b # w) \<in> R \<and> b \<notin> Nt ` As} \<union>
+  {(A,v@w) |A v w. \<exists>B \<in> As. (A,Nt B # w) \<in> R \<and> (B,v) \<in> S}"
 
 lemma derive_expand_iff:
   shows "expand R S As \<turnstile> u \<Rightarrow> v \<longleftrightarrow>
-  (\<exists>u1 u2 A b w. (A, b # w) \<in> R \<and> u = u1 @ NT A # u2 \<and>
-  (b \<notin> NT ` As \<and> v = u1 @ b # w @ u2 \<or>
-  (\<exists>(C,r) \<in> S. C \<in> As \<and> b = NT C \<and> v = u1 @ r @ w @ u2)))"
+  (\<exists>u1 u2 A b w. (A, b # w) \<in> R \<and> u = u1 @ Nt A # u2 \<and>
+  (b \<notin> Nt ` As \<and> v = u1 @ b # w @ u2 \<or>
+  (\<exists>(C,r) \<in> S. C \<in> As \<and> b = Nt C \<and> v = u1 @ r @ w @ u2)))"
   by (fastforce simp: Bex_def expand_def derive_iff split:prod.splits)
 
 definition "expand_list R S As =
-  [(A, b # w). (A, b # w) \<leftarrow> R, b \<notin> NT ` set As] @
-  [(A,v@w). (A, NT B # w) \<leftarrow> R, B \<in> set As, (C,v) \<leftarrow> S, C = B]"
+  [(A, b # w). (A, b # w) \<leftarrow> R, b \<notin> Nt ` set As] @
+  [(A,v@w). (A, Nt B # w) \<leftarrow> R, B \<in> set As, (C,v) \<leftarrow> S, C = B]"
 
 lemma set_expand_list: "set (expand_list R S As) = expand (set R) (set S) (set As)"
   by (auto simp: expand_list_def expand_def)
@@ -308,9 +308,9 @@ definition "unwind_expand'_list R As A A' = (
   let R' = unwind_list R A A' in
   expand_list R' R' (A#As))"
 
-value "unwind_old_expand_list [(2, [NT 1::(int,int)sym])] 1 2"
+value "unwind_old_expand_list [(2, [Nt 1::(int,int)sym])] 1 2"
 
-value "solved_list [(2::int, [NT 2::(int,int)sym, NT 1]), (1, [NT 2])] [1]"
+value "solved_list [(2::int, [Nt 2::(int,int)sym, Nt 1]), (1, [Nt 2])] [1]"
 
 lemma expand_derives_sound:
   assumes ef: "eps_free R"
@@ -330,13 +330,13 @@ next
      apply (rule r_into_rtranclp)
     using derive.intros Un_derive apply fastforce
     subgoal premises Aw  for u1 u2 A w B v
-      apply (rule rtranclp_trans[of _ _ "u1@NT B # w@u2",OF r_into_rtranclp r_into_rtranclp])
+      apply (rule rtranclp_trans[of _ _ "u1@Nt B # w@u2",OF r_into_rtranclp r_into_rtranclp])
       using Aw Un_derive derive.intros apply fastforce
     proof-
       from Aw
-      have "S \<turnstile> u1 @ NT B # w @ u2 \<Rightarrow> u1 @ v @ w @ u2"
+      have "S \<turnstile> u1 @ Nt B # w @ u2 \<Rightarrow> u1 @ v @ w @ u2"
         using derive.simps by fastforce
-      with Aw(1-5) show "R \<union> S \<turnstile> u1 @ NT B # w @ u2 \<Rightarrow> u1 @ v @ w @ u2"
+      with Aw(1-5) show "R \<union> S \<turnstile> u1 @ Nt B # w @ u2 \<Rightarrow> u1 @ v @ w @ u2"
         using Un_derive ef eps_freeE_Cons by fastforce
     qed
     done
@@ -344,7 +344,7 @@ next
 qed
 
 fun leftmost_nt where "leftmost_nt [] = None" |
-"leftmost_nt (NT A # w) = Some A" |
+"leftmost_nt (Nt A # w) = Some A" |
 "leftmost_nt (Tm c # w) = leftmost_nt w"
 
 lemma leftmost_nt_map_Tm_append: "leftmost_nt (map Tm u @ v) = leftmost_nt v"
@@ -382,15 +382,15 @@ proof-
           by (metis Suc Un_derivel zv converse_rtranclp_into_rtranclp less.IH lessI)
       next
         assume "R \<turnstile> u \<Rightarrow>l z"
-        then obtain p A w y2 where [simp]: "u = map Tm p @ NT A # y2"
+        then obtain p A w y2 where [simp]: "u = map Tm p @ Nt A # y2"
           and Aw: "(A,w) \<in> R"
           and [simp]:"z = map Tm p @ w @ y2"
           by (meson derivel.cases)
         with ef obtain a w2 where [simp]: "w = a # w2" by (auto dest: eps_freeE_Cons)
         show ?thesis
-        proof (cases "a \<in> NT ` As")
+        proof (cases "a \<in> Nt ` As")
           case True
-          then obtain B where [simp]: "a = NT B" and B: "B \<in> As" by auto
+          then obtain B where [simp]: "a = Nt B" and B: "B \<in> As" by auto
           from zv B vAs have "m \<noteq> 0"
             apply (intro notI)
             by (auto simp: leftmost_nt_map_Tm_append deriveln_map_Tm_append Cons_eq_map_conv append_eq_map_conv)
@@ -447,7 +447,7 @@ lemma Lang_expand:
 subsection \<open>Soundness of unwind\<close>
 
 lemma unwind_expand':
-  assumes "solved R As" and "A' \<noteq> A" and "A' \<notin> Nt R \<union> As"
+  assumes "solved R As" and "A' \<noteq> A" and "A' \<notin> Nonterminal R \<union> As"
   shows "unwind_expand R As A A' = unwind_expand' R As A A'"
   sorry
 
@@ -455,14 +455,14 @@ lemma eps_free_unwind_new: "eps_free (unwind_new R A A')"
   sorry
 
 lemma in_loop: "(B, w) \<in> loop R A \<longleftrightarrow>
-  A = B \<and> (A,w) \<in> R \<and> (\<exists>w'. w = NT A # w' \<and> w' \<noteq> [])"
+  A = B \<and> (A,w) \<in> R \<and> (\<exists>w'. w = Nt A # w' \<and> w' \<noteq> [])"
   by (auto simp: loop_def)
 
 lemma extract_loop:
-  assumes "R \<turnstile> NT A # u \<Rightarrow>l(n) v" and vA: "\<not>starts_with A v"
+  assumes "R \<turnstile> Nt A # u \<Rightarrow>l(n) v" and vA: "\<not>starts_with A v"
   shows "\<exists>n1 n2 u' w.
     n1 + n2 < n \<and>
-    loop R A \<turnstile> [NT A] \<Rightarrow>l(n1) NT A # u' \<and>
+    loop R A \<turnstile> [Nt A] \<Rightarrow>l(n1) Nt A # u' \<and>
     (A,w) \<in> R \<and> \<not>starts_with A w \<and> R \<turnstile> w@u'@u \<Rightarrow>l(n2) v"
   using assms(1)
 proof (induction n arbitrary: u)
@@ -472,14 +472,14 @@ next
   case (Suc n)
   from Suc.prems
   obtain w where Aw: "(A,w) \<in> R" and wuv: "R \<turnstile> w@u \<Rightarrow>l(n) v"
-    by (auto simp: relpowp_Suc_left derivel_NT_Cons)
+    by (auto simp: relpowp_Suc_left derivel_Nt_Cons)
   show ?case
   proof (cases "starts_with A w")
     case True
-    then obtain w' where [simp]: "w = NT A # w'" by (auto simp: starts_with_iff)
+    then obtain w' where [simp]: "w = Nt A # w'" by (auto simp: starts_with_iff)
     from Suc.IH[OF wuv[simplified]]
     obtain n1 n2 u' x where len: "n1 + n2 < n"
-      and n1: "loop R A \<turnstile> [NT A] \<Rightarrow>l(n1) NT A # u'"
+      and n1: "loop R A \<turnstile> [Nt A] \<Rightarrow>l(n1) Nt A # u'"
       and AxR: "(A, x) \<in> R"
       and Ax: "\<not> starts_with A x"
       and n2: "R \<turnstile> x @ u' @ w' @ u \<Rightarrow>l(n2) v"
@@ -491,9 +491,9 @@ next
     next
       case w': False
       from w' Aw have "(A,w) \<in> loop R A" by (auto simp: in_loop)
-      then have "loop R A \<turnstile> [NT A] \<Rightarrow>l NT A # w'" by (auto simp: derivel_NT_Cons)
+      then have "loop R A \<turnstile> [Nt A] \<Rightarrow>l Nt A # w'" by (auto simp: derivel_Nt_Cons)
       also from deriveln_append[OF n1, of w']
-      have "loop R A \<turnstile> \<dots> \<Rightarrow>l(n1) NT A # u' @ w'" by simp
+      have "loop R A \<turnstile> \<dots> \<Rightarrow>l(n1) Nt A # u' @ w'" by simp
       finally show ?thesis using len AxR Ax n2 by force
     qed
   next
@@ -504,10 +504,10 @@ next
 qed
 
 lemma extract_right_loop:
-  assumes "R \<turnstile> u @ [NT A] \<Rightarrow>r(n) v" and vA: "\<not>ends_with A v"
+  assumes "R \<turnstile> u @ [Nt A] \<Rightarrow>r(n) v" and vA: "\<not>ends_with A v"
   shows "\<exists>n1 n2 u' w.
     n1 + n2 < n \<and>
-    right_loop R A \<turnstile> [NT A] \<Rightarrow>r(n1) u' @ [NT A] \<and>
+    right_loop R A \<turnstile> [Nt A] \<Rightarrow>r(n1) u' @ [Nt A] \<and>
     (A,w) \<in> R \<and> \<not>ends_with A w \<and> R \<turnstile> u@u'@w \<Rightarrow>r(n2) v"
 proof-
   from extract_loop[of n "map_prod id rev ` R" A "rev u" "rev v"] assms
@@ -522,10 +522,10 @@ proof-
 qed
 
 lemma unwind_new_simulate_loop:
-  assumes "loop R A \<turnstile> [NT A] \<Rightarrow>l+ NT A # vs"
-  shows "unwind_new R A A' \<turnstile> [NT A'] \<Rightarrow>* vs"
+  assumes "loop R A \<turnstile> [Nt A] \<Rightarrow>l+ Nt A # vs"
+  shows "unwind_new R A A' \<turnstile> [Nt A'] \<Rightarrow>* vs"
   using assms
-proof (induction "NT A # vs" arbitrary: vs rule: tranclp_induct)
+proof (induction "Nt A # vs" arbitrary: vs rule: tranclp_induct)
   case base
   then show ?case
     apply (intro conjI r_into_rtranclp)
@@ -533,16 +533,16 @@ proof (induction "NT A # vs" arbitrary: vs rule: tranclp_induct)
         derive_singleton)
 next
   case (step y z)
-  then obtain y' where [simp]: "y = NT A # y'"
+  then obtain y' where [simp]: "y = Nt A # y'"
     by (auto simp: derivel_iff in_loop Cons_eq_append_conv)
   from step[simplified]
-  have IH: "unwind_new R A A' \<turnstile> [NT A'] \<Rightarrow>* y'" by auto
-  obtain v where AAv: "(A,NT A # v) \<in> R"
+  have IH: "unwind_new R A A' \<turnstile> [Nt A'] \<Rightarrow>* y'" by auto
+  obtain v where AAv: "(A,Nt A # v) \<in> R"
     and [simp]: "z = v @ y'"
     and v0: "v \<noteq> []"
     using step(2)
     by (auto simp: derivel_iff Cons_eq_append_conv in_loop)
-  from v0 have "(A', v @ [NT A']) \<in> unwind_new R A A'"
+  from v0 have "(A', v @ [Nt A']) \<in> unwind_new R A A'"
       using AAv by (auto simp: unwind_new_def)
   with IH show ?case apply auto
     by (meson converse_rtranclp_into_rtranclp derive_singleton derives_prepend)
@@ -562,7 +562,7 @@ proof (induction n arbitrary: u v rule: less_induct)
   next
     case [simp]: (Suc m)
     with less.prems obtain p B w u' v' where Bw: "(B,w) \<in> R"
-      and [simp]: "u = map Tm p @ NT B # u'" "v = p @ v'"
+      and [simp]: "u = map Tm p @ Nt B # u'" "v = p @ v'"
       and m: "R \<turnstile> w @ u' \<Rightarrow>l(m) map Tm v'"
       apply (auto simp: relpowp_Suc_left derivel_iff[of R u] Cons_eq_append_conv append_eq_Cons_conv
           split: prod.splits)
@@ -570,14 +570,14 @@ proof (induction n arbitrary: u v rule: less_induct)
     show ?thesis
     proof (cases "B = A")
       case [simp]: True
-      have "R \<turnstile> NT A # u' \<Rightarrow>l w @ u'" using Bw
-        by (auto simp: derivel_NT_Cons)
+      have "R \<turnstile> Nt A # u' \<Rightarrow>l w @ u'" using Bw
+        by (auto simp: derivel_Nt_Cons)
       also note m
-      finally have "R \<turnstile> NT A # u' \<Rightarrow>l(n) map Tm v'" by simp
+      finally have "R \<turnstile> Nt A # u' \<Rightarrow>l(n) map Tm v'" by simp
       from extract_loop[OF this]
       obtain n1 n2 u'' w'
         where len: "n1 + n2 < n"
-          and n1: "loop R A \<turnstile> [NT A] \<Rightarrow>l(n1) NT A # u''"
+          and n1: "loop R A \<turnstile> [Nt A] \<Rightarrow>l(n1) Nt A # u''"
           and Aw'R: "(A, w') \<in> R"
           and Aw': "\<not> starts_with A w'"
           and n2: "R \<turnstile> w' @ u'' @ u' \<Rightarrow>l(n2) map Tm v'" by (fastforce simp: starts_with_iff)
@@ -586,27 +586,27 @@ proof (induction n arbitrary: u v rule: less_induct)
       show ?thesis
       proof (cases "n1 > 0")
         case True
-        from Aw' Aw'R have "(A,w'@[NT A']) \<in> unwind R A A'"
+        from Aw' Aw'R have "(A,w'@[Nt A']) \<in> unwind R A A'"
           by (auto simp: unwind_def unwind_old_def)
-        then have "unwind R A A' \<turnstile> u \<Rightarrow> map Tm p @ w' @ NT A' # u'"
+        then have "unwind R A A' \<turnstile> u \<Rightarrow> map Tm p @ w' @ Nt A' # u'"
           by (force simp: derive_iff)
         also have "unwind R A A' \<turnstile> \<dots> \<Rightarrow>* map Tm p @ w' @ u'' @ u'"
         proof (intro derives_prepend)
-          from True n1 have "loop R A \<turnstile> [NT A] \<Rightarrow>l+ NT A # u''"
+          from True n1 have "loop R A \<turnstile> [Nt A] \<Rightarrow>l+ Nt A # u''"
             by (metis tranclp_power)
           from unwind_new_simulate_loop[OF this, of A']
-          have "unwind R A A' \<turnstile> [NT A'] \<Rightarrow>* u''"
+          have "unwind R A A' \<turnstile> [Nt A'] \<Rightarrow>* u''"
             by (metis Un_derive mono_rtranclp unwind_def)
           from derives_append[OF this]
-          show "unwind R A A' \<turnstile> NT A' # u' \<Rightarrow>* u'' @ u'" by simp
+          show "unwind R A A' \<turnstile> Nt A' # u' \<Rightarrow>* u'' @ u'" by simp
         qed
         also have "unwind R A A' \<turnstile> \<dots> \<Rightarrow>* map Tm v"
           by (simp add: IH derives_prepend)
         finally show ?thesis.
       next
         case False
-        from Aw'R Aw' have "unwind R A A' \<turnstile> NT A # u' \<Rightarrow> w' @ u'"
-          by (auto intro!: derivel_imp_derive simp: derivel_NT_Cons unwind_def unwind_old_def)
+        from Aw'R Aw' have "unwind R A A' \<turnstile> Nt A # u' \<Rightarrow> w' @ u'"
+          by (auto intro!: derivel_imp_derive simp: derivel_Nt_Cons unwind_def unwind_old_def)
         with n1 IH False show ?thesis by (auto intro!:derives_prepend)
       qed
     next
@@ -625,7 +625,7 @@ proof (induction n arbitrary: u v rule: less_induct)
 qed
 
 lemma derive_Cons_undef:
-  assumes "a \<notin> NT ` fst ` R"
+  assumes "a \<notin> Nt ` fst ` R"
   shows "R \<turnstile> a # u \<Rightarrow> v \<longleftrightarrow> (\<exists>v'. v = a # v' \<and> R \<turnstile> u \<Rightarrow> v')"
   using assms
   apply (auto simp: derive_iff Cons_eq_append_conv split:prod.splits)
@@ -642,7 +642,7 @@ proof (induction p arbitrary: u v)
   then show ?case by auto
 next
   case (Cons a p)
-  then have "a \<notin> NT ` fst ` R"
+  then have "a \<notin> Nt ` fst ` R"
     by (fastforce simp: image_iff)
   note * = derive_Cons_undef[OF this]
   from Cons.prems have "nt p \<inter> fst ` R = {}" by (auto simp: nt_Cons)
@@ -659,37 +659,37 @@ lemma deriven_append_undef:
 lemma fst_unwind_new: "fst ` unwind_new R A A' \<subseteq> {A'}"
   by (auto simp: unwind_new_def)
 
-lemma NT_in_set_iff_nt: "NT A \<in> set w \<longleftrightarrow> A \<in> nt w"
+lemma Nt_in_set_iff_nt: "Nt A \<in> set w \<longleftrightarrow> A \<in> nt w"
   by (induction w, auto simp: nt_Cons split: sym.splits)
 
 lemma unwind_new_only_last:
-  assumes A'R: "A' \<notin> Nt R"
-    and "unwind_new R A A' \<turnstile> [NT A'] \<Rightarrow>(n) u"
-  shows "NT A' \<notin> set u \<or> (\<exists>u'. u = u' @ [NT A'] \<and> NT A' \<notin> set u')"
+  assumes A'R: "A' \<notin> Nonterminal R"
+    and "unwind_new R A A' \<turnstile> [Nt A'] \<Rightarrow>(n) u"
+  shows "Nt A' \<notin> set u \<or> (\<exists>u'. u = u' @ [Nt A'] \<and> Nt A' \<notin> set u')"
   using assms(2)
 proof (induction n arbitrary: u)
   case 0
   then show ?case by auto
 next
   case (Suc n)
-  from Suc.prems obtain y where A'y: "unwind_new R A A' \<turnstile> [NT A'] \<Rightarrow>(n) y"
+  from Suc.prems obtain y where A'y: "unwind_new R A A' \<turnstile> [Nt A'] \<Rightarrow>(n) y"
     and yu: "unwind_new R A A' \<turnstile> y \<Rightarrow> u"
     by (auto simp: relpowp_Suc_right derive_singleton)
-  from yu have "NT A' \<in> set y" by (auto simp: derive_iff unwind_new_def)
+  from yu have "Nt A' \<in> set y" by (auto simp: derive_iff unwind_new_def)
   with Suc.IH[OF A'y]
-  obtain u' where [simp]: "y = u' @ [NT A']" and A'u': "NT A' \<notin> set u'" by auto
+  obtain u' where [simp]: "y = u' @ [Nt A']" and A'u': "Nt A' \<notin> set u'" by auto
   with yu have "\<exists>v. (A',v) \<in> unwind_new R A A' \<and> u = u' @ v"
     by (auto simp: derive_iff unwind_new_def append_eq_append_conv2
         append_eq_Cons_conv Cons_eq_append_conv)
   with A'R A'u' show ?case
-    by (auto simp: unwind_new_def append_eq_append_conv2 append_eq_Cons_conv Nt_def)
+    by (auto simp: unwind_new_def append_eq_append_conv2 append_eq_Cons_conv Nonterminal_def)
 qed
 
 lemma unwind_new_sound:
-  assumes A'R: "A' \<notin> Nt R"
-    and "unwind_new R A A' \<turnstile> [NT A'] \<Rightarrow>(n) vs"
-    and A'vs: "NT A' \<notin> set vs"
-  shows "R \<turnstile> [NT A] \<Rightarrow>* NT A # vs"
+  assumes A'R: "A' \<notin> Nonterminal R"
+    and "unwind_new R A A' \<turnstile> [Nt A'] \<Rightarrow>(n) vs"
+    and A'vs: "Nt A' \<notin> set vs"
+  shows "R \<turnstile> [Nt A] \<Rightarrow>* Nt A # vs"
   using assms(2-)
 proof (induction n arbitrary: vs)
   case 0
@@ -697,43 +697,43 @@ proof (induction n arbitrary: vs)
 next
   let ?R' = "unwind_new R A A'"
   case (Suc n)
-  then obtain y where y: "?R' \<turnstile> [NT A'] \<Rightarrow> y" 
+  then obtain y where y: "?R' \<turnstile> [Nt A'] \<Rightarrow> y" 
     and yvs: "?R' \<turnstile> y \<Rightarrow>(n) vs" by (auto simp: relpowp_Suc_left)
   show ?case
   proof (cases n)
     case 0
     with yvs have [simp]: "y = vs" by auto
-    with Suc y have "\<exists>v. (A,NT A # v) \<in> R \<and> y = v"
+    with Suc y have "\<exists>v. (A,Nt A # v) \<in> R \<and> y = v"
       apply (simp add: unwind_new_def derive_singleton)
-      by (auto simp: Nt_def split: prod.splits)
+      by (auto simp: Nonterminal_def split: prod.splits)
     then show ?thesis apply (intro r_into_rtranclp)
       by (auto simp: derive_singleton)
   next
     case (Suc m)
-    with yvs have "NT A' \<in> set y"
+    with yvs have "Nt A' \<in> set y"
       by (auto simp: relpowp_Suc_left unwind_new_def derive_iff)
     with A'R y obtain v
-      where AAv: "(A,NT A # v) \<in> R" and [simp]: "y = v @ [NT A']"
-      by (auto simp: unwind_new_def derive_singleton Nt_def split: prod.splits)
-    from AAv A'R have A'v: "NT A' \<notin> set v" by (auto simp: Nt_def)
+      where AAv: "(A,Nt A # v) \<in> R" and [simp]: "y = v @ [Nt A']"
+      by (auto simp: unwind_new_def derive_singleton Nonterminal_def split: prod.splits)
+    from AAv A'R have A'v: "Nt A' \<notin> set v" by (auto simp: Nonterminal_def)
     with fst_unwind_new[of R A A']
-    have "nt v \<inter> fst ` ?R' = {}" by (auto simp: NT_in_set_iff_nt)
+    have "nt v \<inter> fst ` ?R' = {}" by (auto simp: Nt_in_set_iff_nt)
     from yvs[simplified] deriven_append_undef[OF this]
-    obtain w where [simp]: "vs = v @ w" and A'w: "?R' \<turnstile> [NT A'] \<Rightarrow>(n) w"
+    obtain w where [simp]: "vs = v @ w" and A'w: "?R' \<turnstile> [Nt A'] \<Rightarrow>(n) w"
       by blast
-    have "NT A' \<notin> set w" using Suc.prems(2) by auto
+    have "Nt A' \<notin> set w" using Suc.prems(2) by auto
     note Suc.IH[OF A'w this]
-    also have "R \<turnstile> NT A # w \<Rightarrow> NT A # vs"
-      using AAv derivel_NT_Cons derivel_imp_derive by fastforce
+    also have "R \<turnstile> Nt A # w \<Rightarrow> Nt A # vs"
+      using AAv derivel_Nt_Cons derivel_imp_derive by fastforce
     finally show ?thesis.
   qed
 qed
 
 lemma right_loop_unwind:
-  assumes A'R: "A' \<notin> Nt R"
+  assumes A'R: "A' \<notin> Nonterminal R"
   shows "right_loop (unwind R A A') A' \<subseteq> unwind_new R A A'"
   using assms
-  by (auto simp: right_loop_def unwind_def unwind_old_def unwind_new_def Nt_def)
+  by (auto simp: right_loop_def unwind_def unwind_old_def unwind_new_def Nonterminal_def)
 
 lemma map_Tm_eq_map_Tm: "map Tm u = map Tm v \<longleftrightarrow> u = v"
   by (metis list.inj_map_strong sym.inject(2))
@@ -743,9 +743,9 @@ lemma deriver_mono: "R \<subseteq> S \<Longrightarrow> deriver R \<le> deriver S
 
 lemma unwind_sound:
   assumes "unwind R A A' \<turnstile> u \<Rightarrow>r(n) v"
-    and "NT A' \<notin> set u"
-    and "NT A' \<notin> set v"
-    and A'R: "A' \<notin> Nt R"
+    and "Nt A' \<notin> set u"
+    and "Nt A' \<notin> set v"
+    and A'R: "A' \<notin> Nonterminal R"
   shows "R \<turnstile> u \<Rightarrow>* v"
   using assms(1-3)
 proof (induction n arbitrary: u v rule: less_induct)
@@ -758,52 +758,52 @@ proof (induction n arbitrary: u v rule: less_induct)
     case [simp]: (Suc m)
     from less.prems obtain B w l r
       where BwR': "(B,w) \<in> unwind_old R A A'"
-        and [simp]: "u = l @ NT B # map Tm r"
+        and [simp]: "u = l @ Nt B # map Tm r"
         and m: "unwind R A A' \<turnstile> l @ w @ map Tm r \<Rightarrow>r(m) v"
       by (auto simp: relpowp_Suc_left append_eq_append_conv2 unwind_def unwind_new_def
           dest!:deriver_iff[THEN iffD1])
     from less.prems
-    have A'l: "NT A' \<notin> set l" by auto
+    have A'l: "Nt A' \<notin> set l" by auto
     show ?thesis
-    proof (cases "NT A' \<in> set w")
+    proof (cases "Nt A' \<in> set w")
       case True
       with BwR' A'R obtain w'
-        where [simp]: "B = A" "w = w' @ [NT A']"
-          and Aw'R: "(A,w') \<in> R" and A'w': "NT A' \<notin> set w'"
-        by (auto simp: unwind_old_def Nt_def split: prod.splits)
+        where [simp]: "B = A" "w = w' @ [Nt A']"
+          and Aw'R: "(A,w') \<in> R" and A'w': "Nt A' \<notin> set w'"
+        by (auto simp: unwind_old_def Nonterminal_def split: prod.splits)
       from m[folded append_assoc, unfolded derivern_append_map_Tm]
-      obtain v' where v': "unwind R A A' \<turnstile> (l @ w') @ [NT A'] \<Rightarrow>r(m) v'"
+      obtain v' where v': "unwind R A A' \<turnstile> (l @ w') @ [Nt A'] \<Rightarrow>r(m) v'"
         and [simp]: "v = v' @ map Tm r"
         by auto
       from less.prems have "\<not>ends_with A' v'" by (auto simp: ends_with_def)
       from extract_right_loop[OF v' this]
       obtain n1 n2 u' w'' where len: "n1 + n2 < m"
-        and n1: "right_loop (unwind R A A') A' \<turnstile> [NT A'] \<Rightarrow>r(n1) u' @ [NT A']"
+        and n1: "right_loop (unwind R A A') A' \<turnstile> [Nt A'] \<Rightarrow>r(n1) u' @ [Nt A']"
         and w'': "(A', w'') \<in> unwind R A A'" "\<not> ends_with A' w''"
         and n2: "unwind R A A' \<turnstile> (l @ w') @ u' @ w'' \<Rightarrow>r(n2) v'" by auto
       from w'' A'R have A'w''R: "(A',w'') \<in> unwind_new R A A'"
-        and A'w'': "NT A' \<notin> set w''"
-        by (auto simp: unwind_def unwind_old_def unwind_new_def Nt_def ends_with_def)
+        and A'w'': "Nt A' \<notin> set w''"
+        by (auto simp: unwind_def unwind_old_def unwind_new_def Nonterminal_def ends_with_def)
       from n1 right_loop_unwind[OF A'R, THEN deriver_mono]
-      have n1: "unwind_new R A A' \<turnstile> [NT A'] \<Rightarrow>r(n1) u' @ [NT A']"
+      have n1: "unwind_new R A A' \<turnstile> [Nt A'] \<Rightarrow>r(n1) u' @ [Nt A']"
         apply (auto simp: le_fun_def)
         by (metis relpowp_mono)
       from unwind_new_only_last[OF A'R derivern_imp_deriven[OF n1]]
-      have A'u': "NT A' \<notin> set u'" by auto
+      have A'u': "Nt A' \<notin> set u'" by auto
       note n1
-      also have "unwind_new R A A' \<turnstile> u' @ [NT A'] \<Rightarrow>r u' @ w''"
-        using A'w''R by (auto simp: deriver_snoc_NT simp del: append_assoc)
-      finally have "unwind_new R A A' \<turnstile> [NT A'] \<Rightarrow>(Suc n1) u' @ w''"
+      also have "unwind_new R A A' \<turnstile> u' @ [Nt A'] \<Rightarrow>r u' @ w''"
+        using A'w''R by (auto simp: deriver_snoc_Nt simp del: append_assoc)
+      finally have "unwind_new R A A' \<turnstile> [Nt A'] \<Rightarrow>(Suc n1) u' @ w''"
         by (rule derivern_imp_deriven)
       from unwind_new_sound[OF A'R this] A'u' A'w' A'w''
-      have "R \<turnstile> [NT A] \<Rightarrow>* NT A # u' @ w''" by auto
+      have "R \<turnstile> [Nt A] \<Rightarrow>* Nt A # u' @ w''" by auto
       also have "R \<turnstile> \<dots> \<Rightarrow> w' @ u' @ w''" using Aw'R
-        by (auto intro!: derivel_imp_derive simp: derivel_NT_Cons)
-      finally have "R \<turnstile> [NT A] \<Rightarrow>* \<dots>".
+        by (auto intro!: derivel_imp_derive simp: derivel_Nt_Cons)
+      finally have "R \<turnstile> [Nt A] \<Rightarrow>* \<dots>".
       note derives_prepend[OF this]
       also from A'u' A'w' A'w'' less.prems(2-3) less.IH[OF _ n2] len
       have "R \<turnstile> l @ w' @ u' @ w'' \<Rightarrow>* v'" by auto
-      finally have "R \<turnstile> l @ [NT A] \<Rightarrow>* v'".
+      finally have "R \<turnstile> l @ [Nt A] \<Rightarrow>* v'".
       from derives_append[OF this]
       show ?thesis by simp
     next
@@ -812,14 +812,14 @@ proof (induction n arbitrary: u v rule: less_induct)
       then have "R \<turnstile> u \<Rightarrow> l @ w @ map Tm r" by (auto simp: derive_iff)
       also have "R \<turnstile> \<dots> \<Rightarrow>* v"
         apply (rule less.IH[OF _ m]) using A'R BwR' A'l False less.prems
-        by (auto simp: Nt_def split:prod.splits)
+        by (auto simp: Nonterminal_def split:prod.splits)
       finally show ?thesis.
     qed
   qed
 qed
 
 lemma unwind_derives:
-  assumes "NT A' \<notin> set u" and "A' \<notin> Nt R"
+  assumes "Nt A' \<notin> set u" and "A' \<notin> Nonterminal R"
   shows "unwind R A A' \<turnstile> u \<Rightarrow>* map Tm v \<longleftrightarrow> R \<turnstile> u \<Rightarrow>* map Tm v"
     (is "?l \<longleftrightarrow> ?r")
 proof
@@ -839,7 +839,7 @@ next
 qed
 
 lemma Lang_unwind:
-  assumes A'R: "A' \<notin> Nt R" and "B \<noteq> A'"
+  assumes A'R: "A' \<notin> Nonterminal R" and "B \<noteq> A'"
   shows "Lang (unwind R A A') B = Lang R B"
   apply (rule Lang_eqI_derives)
   apply (rule unwind_derives)
@@ -917,12 +917,12 @@ lemma unwind_derives:
 
 lemma Lang_unwind_expand:
   assumes ef: "eps_free R"
-  assumes "solved R As" and "A' \<noteq> A" and A'RAs: "A' \<notin> Nt R \<union> As"
+  assumes "solved R As" and "A' \<noteq> A" and A'RAs: "A' \<notin> Nonterminal R \<union> As"
     and "A' \<noteq> B"
   shows "Lang (unwind_expand R As A A') B = Lang R B"
   apply (simp add: unwind_expand_def Let_def del:)
   apply (subst Lang_expand[OF eps_free_unwind_new])
-  using A'RAs apply (force simp: unwind_new_def Nt_def)
+  using A'RAs apply (force simp: unwind_new_def Nonterminal_def)
   using Lang_unwind
   apply (auto simp:  )
   sorry
@@ -933,9 +933,9 @@ lemma eps_free_unwind_old_expand_list:
   using assms
   by (auto simp: unwind_old_expand_def eps_free_def)
 
-lemma in_Nt_if_starts_with: "(A, w) \<in> R \<Longrightarrow> starts_with B w \<Longrightarrow> B \<in> Nt R"
+lemma in_Nonterminal_if_starts_with: "(A, w) \<in> R \<Longrightarrow> starts_with B w \<Longrightarrow> B \<in> Nonterminal R"
   apply (cases "(B,w)" rule: starts_with.cases)
-    apply (auto simp: Nt_def split: prod.split)
+    apply (auto simp: Nonterminal_def split: prod.split)
   by (metis list.set_intros(1) prod.inject)
   
 lemma loop_free_unwind_old_expand:
@@ -961,7 +961,7 @@ lemma loop_free_unwind_new_list:
   shows "loop_free (unwind_new R A A') A"
   using assms by (auto simp: loop_free_def starts_with_iff unwind_new_def Cons_eq_append_conv)
 
-definition Rhs1s where "Rhs1s R = [A. (B, NT A # w) \<leftarrow> R]"
+definition Rhs1s where "Rhs1s R = [A. (B, Nt A # w) \<leftarrow> R]"
 
 lemma set_Rhs1s: "set (Rhs1s R) = Rhs1 (set R)"
   by (auto simp: Rhs1s_def Rhs1_def Lnt_def rhs1_def image_Collect)
@@ -970,13 +970,13 @@ definition "eps_free_list R = (\<forall>(A,w) \<in> set R. w \<noteq> [])"
 
 definition Rex :: "(int,int) prod list"
   where "Rex = [
-  (1,[NT 2, NT 2]), (1, [Tm 0]),
-  (2, [NT 2, NT 2, NT 2]), (2, [Tm 0, NT 2]), (2, [Tm 1])]"
+  (1,[Nt 2, Nt 2]), (1, [Tm 0]),
+  (2, [Nt 2, Nt 2, Nt 2]), (2, [Tm 0, Nt 2]), (2, [Tm 1])]"
 
 definition Rex2 :: "(int,int) prod list"
   where "Rex2 = [
-  (1, [NT 2, Tm 0]),
-  (2, [NT 1, Tm 2]), (2, [Tm 1, NT 1]), (2, [Tm 3])]"
+  (1, [Nt 2, Tm 0]),
+  (2, [Nt 1, Tm 2]), (2, [Tm 1, Nt 1]), (2, [Tm 3])]"
 
 value "unwind_list Rex 2 3"
 
@@ -1026,7 +1026,7 @@ lemma expand_list_solved_list2:
       split: prod.splits)
 
 definition Rex3 :: "(int,int) prod list" where "Rex3 = [
-(0,[NT 0]), (1,[NT 1, NT 0])]"
+(0,[Nt 0]), (1,[Nt 1, Nt 0])]"
 
 value "unwind_new_list Rex3 1 2"
 
@@ -1035,18 +1035,18 @@ value "expand_list (unwind_new_list Rex3 1 2) (unwind_old_expand_list Rex3 1 2) 
 text \<open>The following is true without assuming solved_listness of \<open>As\<close>,
 because of the definition of \<open>expand\<close>.\<close>
 
-lemma hd_in_Nt: "(A,NT B#w) \<in> R \<Longrightarrow> B \<in> Nt R"
-  apply (auto simp: Nt_def split: prod.splits)
+lemma hd_in_Nonterminal: "(A,Nt B#w) \<in> R \<Longrightarrow> B \<in> Nonterminal R"
+  apply (auto simp: Nonterminal_def split: prod.splits)
   by (metis list.set_intros(1) prod.inject)
 
-lemma hd2_in_Nt: "(A,x#NT B#w) \<in> R \<Longrightarrow> B \<in> Nt R"
-  apply (auto simp: Nt_def split: prod.splits)
+lemma hd2_in_Nonterminal: "(A,x#Nt B#w) \<in> R \<Longrightarrow> B \<in> Nonterminal R"
+  apply (auto simp: Nonterminal_def split: prod.splits)
   by (metis list.set_intros(1,2) prod.inject)
   
 
 lemma solved_list_expand_list_unwind_new_list:
   assumes "A' \<notin> As"
-    and "eps_free R" "A' \<notin> Nt R"
+    and "eps_free R" "A' \<notin> Nonterminal R"
     and "solved R As"
   shows "solved (expand (unwind_new R A A')
  (unwind_old_expand R A A') (insert A As))
@@ -1055,20 +1055,20 @@ lemma solved_list_expand_list_unwind_new_list:
   apply (intro solvedI)
   by (auto simp: expand_def solved_not
       unwind_new_def unwind_old_expand_def neq_Nil_conv starts_with_iff
-      Cons_eq_append_conv eps_free_Nil hd_in_Nt hd2_in_Nt)
+      Cons_eq_append_conv eps_free_Nil hd_in_Nonterminal hd2_in_Nonterminal)
 
 
 text \<open>Instead, preservation of the language requires solved_listness
 of \<open>R\<close> with respect to \<open>As\<close>.\<close>
 
 lemma solved_unwind_expand:
-  assumes ef: "eps_free R" and A': "A' \<notin> Nt R \<union> As"
+  assumes ef: "eps_free R" and A': "A' \<notin> Nonterminal R \<union> As"
     and so: "solved R As"
   shows "solved (unwind_expand R As A A') (insert A (insert A' As))"
 proof-
   have so2: "solved R (insert A' As)"
     using so A' 
-    by (auto simp: solved_def in_Nt_if_starts_with split: prod.splits)
+    by (auto simp: solved_def in_Nonterminal_if_starts_with split: prod.splits)
   show ?thesis
     apply (auto simp: unwind_expand_def solved_Un
         solved_unwind_old_expand[OF so2 ef])
@@ -1136,13 +1136,13 @@ fun realtime where
 end
 
 lemma solved_if_disj:
-  assumes disj: "set As' \<inter> Nt R = {}"
+  assumes disj: "set As' \<inter> Nonterminal R = {}"
   shows "solved R (set As')"
   using disj
-  by (auto simp: solved_def dest:in_Nt_if_starts_with)
+  by (auto simp: solved_def dest:in_Nonterminal_if_starts_with)
 
 
-lemma Nt_realtime: "Nt (realtime R As As') \<subseteq> Nt R \<union> set As \<union> set As'"
+lemma Nonterminal_realtime: "Nonterminal (realtime R As As') \<subseteq> Nonterminal R \<union> set As \<union> set As'"
   sorry
 
 context
@@ -1166,12 +1166,12 @@ qed
 lemma solved_realtime:
   assumes "eps_free R"
     and "length As \<le> length As'"
-    and "distinct (As @ As')" and "set As' \<inter> Nt R = {}"
+    and "distinct (As @ As')" and "set As' \<inter> Nonterminal R = {}"
   shows "solved (realtime R As As') (set As \<union> set As')"
   using assms
 proof (induction As As' rule: realtime.induct)
   case (1 A As A' As')
-  with Nt_realtime[of R]
+  with Nonterminal_realtime[of R]
     solved_unwind_expand[where A=A and A'=A' and As = "set As \<union> set As'" and R ="realtime R As As'"]
   show ?case by (auto intro!: simp: eps_free_realtime insert_commute) 
 next
@@ -1185,13 +1185,13 @@ qed
 lemma Lang_realtime:
   assumes "eps_free R"
     and "length As \<le> length As'"
-    and "distinct (As @ As')" and "set As' \<inter> Nt R = {}"
+    and "distinct (As @ As')" and "set As' \<inter> Nonterminal R = {}"
     and "B \<notin> set As'"
   shows "Lang (realtime R As As') B = Lang R B"
   using assms(2-)
 proof (induction As As' rule: realtime.induct)
   case (1 A As A' As')
-  with Nt_realtime[of R] solved_realtime[OF \<open>eps_free R\<close> ]
+  with Nonterminal_realtime[of R] solved_realtime[OF \<open>eps_free R\<close> ]
     Lang_unwind_expand[where A=A and A'=A' and As = "set As \<union> set As'" and R ="realtime R As As'" and B=B]
   show ?case by (auto intro!: simp: eps_free_realtime insert_commute) 
 next
